Risc0/Cirgen/Defs.lean
@@ -31,6 +31,10 @@ namespace Risc0
     | GetGlobal : BufferVar → ℕ        → Op x
     | Slice     : BufferVar → ℕ    → ℕ → Op x
 
+  @[default_instance] noncomputable
+  instance : SizeOf (Op x) where
+    sizeOf _ := 1
+
   def isGetValid (st : State) (buf : BufferVar) (back : Back) (offset : ℕ) :=
     back ≤ st.cycle ∧
     buf ∈ st.vars ∧
@@ -101,13 +105,184 @@ namespace Risc0
     | Eqz       : FeltVar                → MLIR x
     | If        : FeltVar       → MLIR x → MLIR x
     | Nondet    : MLIR InNondet          → MLIR NotInNondet
+    | Noop      :                          MLIR x
     | Sequence  : MLIR x        → MLIR x → MLIR x
     -- Ops
+    | Barrier   :                           MLIR x
     | Fail      :                           MLIR x
     | Set       : BufferVar → ℕ → FeltVar → MLIR InNondet
     | SetGlobal : BufferVar → ℕ → FeltVar → MLIR InNondet
+    -- Extern
+        -- Extern
+    | PlonkAccumRead  : BufferVar → ℕ                → MLIR InNondet
+    | PlonkAccumWrite : BufferVar → List FeltVar → ℕ → MLIR InNondet
+    | PlonkRead       : BufferVar → ℕ                → MLIR InNondet
+    | PlonkWrite      : BufferVar → List FeltVar → ℕ → MLIR InNondet
 
   abbrev MLIRProgram := MLIR NotInNondet
+
+  inductive ExternPlonkBuffer | PlonkRows | PlonkAccumRows
+  deriving DecidableEq
+
+  @[simp]
+  lemma sizeOf_ExternPlonkBuffer {x : ExternPlonkBuffer} : sizeOf x = 1 := by
+    cases x <;> simp
+
+  instance : ToString ExternPlonkBuffer := ⟨
+    (match · with | .PlonkRows => "PlonkRows" | .PlonkAccumRows => "PlonkAccumRows")
+  ⟩
+
+  def mangle (table : ExternPlonkBuffer) (discr : BufferVar) : String :=
+    toString table ++ discr.name
+
+  namespace MLIR.ExternOp
+    section
+
+      variable (buf : BufferVar) (args : List FeltVar) (outCount : ℕ)
+
+      def memoryName (mangledName : String) := "mem" ++ mangledName
+
+      def plonkExternWrite (discr : ExternPlonkBuffer) (st : State) : State := 
+        let mangledName := mangle discr buf
+        if outCount = 0
+        then st.allocateBufferRow! ⟨mangledName⟩ args.length |>.setMany! ⟨mangledName⟩ args
+             |>.allocateBufferRow! ⟨memoryName mangledName⟩ 1 |>.set! ⟨memoryName mangledName⟩ 0 0
+        else {st with isFailed := true}
+
+      def getSequence_aux (discr : ExternPlonkBuffer) (offset : ℕ) : ℕ → MLIR .InNondet
+        | 0 => Noop
+        | k + 1 => Sequence
+                     (Assign s!"{mangle discr buf}#{k}" (Op.Get ⟨mangle discr buf⟩ offset k))
+                     (getSequence_aux discr offset k)
+
+      def getSequence (discr : ExternPlonkBuffer) (offset : ℕ) :=
+        getSequence_aux buf discr offset outCount
+
+      def getOffset (discr : ExternPlonkBuffer) : MLIR x :=
+        Assign s!"mem{mangle discr buf}" (Op.Get ⟨s!"mem{mangle discr buf}"⟩ 0 0)
+
+      @[simp]
+      lemma getSequence_aux_succ :
+        getSequence_aux buf discr offset k.succ =
+        Sequence (Assign s!"{mangle discr buf}#{k}" (Op.Get ⟨mangle discr buf⟩ offset k)) (getSequence_aux buf discr offset k) := rfl
+
+      abbrev plonkExternRead (discr : ExternPlonkBuffer) (offset : ℕ) : MLIR .InNondet :=
+        getSequence buf outCount discr offset
+
+      def memoryFor (mangledName : String) (st : State) :=
+        (st.buffers[(⟨memoryName mangledName⟩ : BufferVar)].get![0]!)[0]!.get!.val
+
+      def plonkRead (discr : ExternPlonkBuffer) (st : State) :=
+        let offset := memoryFor (mangle discr buf) st
+        if st.buffers[(⟨mangle discr buf⟩ : BufferVar)].get![offset]!.length = outCount ∧
+           ⟨mangle discr buf⟩ ∈ st.buffers
+        then ExternOp.plonkExternRead buf outCount discr offset
+        else Fail
+
+      def plonkReadBump (discr : ExternPlonkBuffer) (st : State) : State :=
+        let buffer := mangle discr buf
+        st.set! ⟨memoryName buffer⟩ 0 (memoryFor buffer st)
+
+      -- Note: In theory, this can tag a non-special table if they happen to be called like this.
+      -- We'll need a more robust system should we want to extend this further.
+      def isSpecial (buf : BufferVar) :=
+        buf.name.startsWith (toString ExternPlonkBuffer.PlonkRows) ||
+        buf.name.startsWith (toString ExternPlonkBuffer.PlonkAccumRows)
+
+      def sortPlonkBuffers (st : State) : State :=
+        let specialNames := st.vars.filter isSpecial
+        specialNames.foldr (init := st)
+          λ name acc ↦
+            {acc with buffers := acc.buffers[name] ←ₘ acc.buffers[name].get!.sort}
+
+    end
+  end MLIR.ExternOp  
+
+  @[simp]
+  lemma sizeOf_Variable {x : Variable α} : SizeOf.sizeOf x = 1 + SizeOf.sizeOf x.name := by cases x; simp
+
+  @[simp]
+  lemma sizeOf_IsNondet {x : IsNondet} : SizeOf.sizeOf x = 1 := by cases x <;> simp
+
+  @[default_instance] noncomputable
+  instance : SizeOf (MLIR x) where
+    sizeOf command := let rec go {x} : MLIR x → ℕ
+      | .Assign _ _ => 1
+      | .Barrier => 1
+      | .DropFelt _ => 1
+      | .Eqz _ => 1
+      | .If _ prog => 1 + go prog
+      | .Nondet block => 1 + go block
+      | .Noop => 0
+      | .Sequence a b => 1 + go a + go b
+      -- Ops
+      | .Fail => 0
+      | .Set _ _ _ => 1
+      | .SetGlobal _ _ _ => 1
+      -- Extern
+      | .PlonkAccumRead _ n => 1 + n + n
+      | .PlonkAccumWrite _ _ _ => 1
+      | .PlonkRead _ n => 1 + n + n
+      | .PlonkWrite _ _ _ => 1
+    go command
+
+  @[simp]
+  lemma sizeOf_ExternOp_zero :
+    sizeOf (MLIR.ExternOp.plonkExternRead buf 0 discr offset) = 0 := by
+    simp [sizeOf, instSizeOfMLIR.go]
+
+  @[simp]
+  lemma sizeOf_ExternOp_succ :
+    sizeOf (MLIR.ExternOp.plonkExternRead buf (Nat.succ k) discr offset) = 
+    sizeOf (MLIR.ExternOp.plonkExternRead buf k discr offset) + 2 := by
+    simp_arith [sizeOf, instSizeOfMLIR.go]
+    rfl
+      
+  @[simp]
+  lemma sizeOf_PlonkAccumRead_zero :
+    sizeOf (MLIR.PlonkAccumRead buf 0) = 1 := by
+    simp [sizeOf, instSizeOfMLIR.go]
+
+  @[simp]
+  lemma sizeOf_PlonkAccumRead_succ :
+    sizeOf (MLIR.PlonkAccumRead buf (Nat.succ k)) = 
+    sizeOf (MLIR.PlonkAccumRead buf k) + 2 := by
+    simp_arith [sizeOf, instSizeOfMLIR.go]
+
+  @[simp]
+  lemma sizeOf_PlonkRead_zero :
+    sizeOf (MLIR.PlonkRead buf 0) = 1 := by
+    simp [sizeOf, instSizeOfMLIR.go]
+
+  @[simp]
+  lemma sizeOf_PlonkRead_succ :
+    sizeOf (MLIR.PlonkRead buf (Nat.succ k)) = 
+    sizeOf (MLIR.PlonkRead buf k) + 2 := by
+    simp_arith [sizeOf, instSizeOfMLIR.go]
+
+  lemma sizeOf_plonkExternRead_lt_sizeOf_plonkAccumRead :
+    sizeOf (MLIR.ExternOp.plonkExternRead buf outCount discr offset) <
+    sizeOf (MLIR.PlonkAccumRead buf outCount) := by
+    induction outCount <;> simp [*]
+
+  lemma sizeOf_plonkExternRead_lt_sizeOf_plonkRead :
+    sizeOf (MLIR.ExternOp.plonkExternRead buf outCount discr offset) <
+    sizeOf (MLIR.PlonkRead buf outCount) := by
+    induction outCount <;> simp [*]
+
+  lemma sizeOf_plonkRead_lt_sizeOf_plonkAccumRead :
+    sizeOf (MLIR.ExternOp.plonkRead buf outCount discr st) <
+    sizeOf (MLIR.PlonkAccumRead buf outCount) := by
+    simp [MLIR.ExternOp.plonkRead]; split_ifs
+    · exact sizeOf_plonkExternRead_lt_sizeOf_plonkAccumRead
+    · simp [sizeOf, instSizeOfMLIR.go]
+
+  lemma sizeOf_plonkRead_lt_sizeOf_plonkRead :
+    sizeOf (MLIR.ExternOp.plonkRead buf outCount discr st) <
+    sizeOf (MLIR.PlonkRead buf outCount) := by
+    simp [MLIR.ExternOp.plonkRead]; split_ifs
+    · exact sizeOf_plonkExternRead_lt_sizeOf_plonkRead
+    · simp [sizeOf, instSizeOfMLIR.go]
 
   -- Step through the entirety of a `MLIR` MLIR program from initial state
   -- `state`, yielding the post-execution state and possibly a constraint
@@ -115,18 +290,41 @@ namespace Risc0
   def MLIR.run {α : IsNondet} (program : MLIR α) (st : State) : State :=
     match program with
       -- Meta
-      -- | Assign name op => st[name] ←ₛ Γ st ⟦op⟧ₑ
       | Assign name op => st.update name (op.eval st)
       | DropFelt k     => .dropFelts st k
       | Eqz x          => withEqZero st.felts[x]!.get! st
-      | If x program   => if st.felts[x]!.get! = 0 then st else program.run st
-      | Nondet block   => block.run st
-      | Sequence a b   => b.run (a.run st)
+      | If x prog   =>
+          if st.felts[x]!.get! = 0 then st else prog.run st
+      | Nondet block   =>
+          block.run st
+      | Noop           => st
+      | Sequence a b   =>
+          have : sizeOf a < sizeOf (Sequence a b) := by
+            cases a <;> simp [sizeOf, instSizeOfMLIR.go] <;> linarith
+          have : sizeOf b < sizeOf (Sequence a b) := by
+            cases b <;> simp [sizeOf, instSizeOfMLIR.go]
+          b.run (a.run st)
       -- Ops
+      | Barrier                  => ExternOp.sortPlonkBuffers st
       | Fail                     => {st with isFailed := true}
       | Set buf offset val       => st.set! buf offset st.felts[val]!.get!
       | SetGlobal buf offset val => st.setGlobal! buf offset st.felts[val]!.get! -- Behind the scenes setGlobal actually flattens a 2d buffer into a 1d buffer
-                                                                                -- and indexes into it. This is a side effect of global buffers only being 1d anyway
+                                                                                 -- and indexes into it. This is a side effect of global buffers only being 1d anyway
+      -- Extern
+      | PlonkAccumRead buf outCount =>
+        ExternOp.plonkReadBump buf .PlonkAccumRows <|
+          ExternOp.plonkRead buf outCount .PlonkAccumRows st |>.run st
+      | PlonkAccumWrite buf args outCount => ExternOp.plonkExternWrite buf args outCount .PlonkAccumRows st
+      | PlonkRead buf outCount =>
+        ExternOp.plonkReadBump buf .PlonkRows <|
+          ExternOp.plonkRead buf outCount .PlonkRows st |>.run st
+      | PlonkWrite buf args outCount => ExternOp.plonkExternWrite buf args outCount .PlonkRows st
+  termination_by run _ program st => sizeOf program
+  decreasing_by simp_wf
+                all_goals try (simp [sizeOf, instSizeOfMLIR.go]; done)
+                all_goals try (cases a <;> simp [sizeOf, instSizeOfMLIR.go] <;> try linarith)
+                all_goals try apply sizeOf_plonkRead_lt_sizeOf_plonkAccumRead
+
 
   @[simp]
   abbrev MLIR.runProgram (program : MLIRProgram) := program.run
