Risc0.lean
@@ -7,183 +7,167 @@ import Risc0.MlirTactics
 import Risc0.Optimisation
 import Risc0.Wheels
 
-import Risc0.Gadgets.OneHot20.Witness.Code
-import Risc0.Gadgets.OneHot20.Constraints.Code
-import Risc0.Gadgets.OneHot20.Constraints.CodeReordered
-import Risc0.Gadgets.OneHot20.Witness.CodeReordered
-import Risc0.Gadgets.OneHot20.Constraints.CodeParts
-import Risc0.Gadgets.OneHot20.Witness.CodeParts
-import Risc0.Gadgets.OneHot20.Constraints.CodeDrops
-import Risc0.Gadgets.OneHot20.Witness.CodeDrops
-import Risc0.Gadgets.OneHot20.Constraints.WeakestPresPart0
-import Risc0.Gadgets.OneHot20.Constraints.WeakestPresPart1
-import Risc0.Gadgets.OneHot20.Constraints.WeakestPresPart2
-import Risc0.Gadgets.OneHot20.Constraints.WeakestPresPart3
-import Risc0.Gadgets.OneHot20.Constraints.WeakestPresPart4
-import Risc0.Gadgets.OneHot20.Constraints.WeakestPresPart5
-import Risc0.Gadgets.OneHot20.Constraints.WeakestPresPart6
-import Risc0.Gadgets.OneHot20.Constraints.WeakestPresPart7
-import Risc0.Gadgets.OneHot20.Constraints.WeakestPresPart8
-import Risc0.Gadgets.OneHot20.Constraints.WeakestPresPart9
-import Risc0.Gadgets.OneHot20.Constraints.WeakestPresPart10
-import Risc0.Gadgets.OneHot20.Constraints.WeakestPresPart11
-import Risc0.Gadgets.OneHot20.Constraints.WeakestPresPart12
-import Risc0.Gadgets.OneHot20.Constraints.WeakestPresPart13
-import Risc0.Gadgets.OneHot20.Constraints.WeakestPresPart14
-import Risc0.Gadgets.OneHot20.Constraints.WeakestPresPart15
-import Risc0.Gadgets.OneHot20.Constraints.WeakestPresPart16
-import Risc0.Gadgets.OneHot20.Constraints.WeakestPresPart17
-import Risc0.Gadgets.OneHot20.Constraints.WeakestPresPart18
-import Risc0.Gadgets.OneHot20.Constraints.WeakestPresPart19
-import Risc0.Gadgets.OneHot20.Constraints.WeakestPresPart20
-import Risc0.Gadgets.OneHot20.Constraints.WeakestPresPart21
-import Risc0.Gadgets.OneHot20.Constraints.WeakestPresPart22
-import Risc0.Gadgets.OneHot20.Constraints.WeakestPresPart23
-import Risc0.Gadgets.OneHot20.Constraints.WeakestPresPart24
-import Risc0.Gadgets.OneHot20.Constraints.WeakestPresPart25
-import Risc0.Gadgets.OneHot20.Constraints.WeakestPresPart26
-import Risc0.Gadgets.OneHot20.Constraints.WeakestPresPart27
-import Risc0.Gadgets.OneHot20.Constraints.WeakestPresPart28
-import Risc0.Gadgets.OneHot20.Constraints.WeakestPresPart29
-import Risc0.Gadgets.OneHot20.Constraints.WeakestPresPart30
-import Risc0.Gadgets.OneHot20.Constraints.WeakestPresPart31
-import Risc0.Gadgets.OneHot20.Constraints.WeakestPresPart32
-import Risc0.Gadgets.OneHot20.Constraints.WeakestPresPart33
-import Risc0.Gadgets.OneHot20.Constraints.WeakestPresPart34
-import Risc0.Gadgets.OneHot20.Constraints.WeakestPresPart35
-import Risc0.Gadgets.OneHot20.Constraints.WeakestPresPart36
-import Risc0.Gadgets.OneHot20.Constraints.WeakestPresPart37
-import Risc0.Gadgets.OneHot20.Constraints.WeakestPresPart38
-import Risc0.Gadgets.OneHot20.Constraints.WeakestPresPart39
-import Risc0.Gadgets.OneHot20.Witness.WeakestPresPart0
-import Risc0.Gadgets.OneHot20.Witness.WeakestPresPart1
-import Risc0.Gadgets.OneHot20.Witness.WeakestPresPart2
-import Risc0.Gadgets.OneHot20.Witness.WeakestPresPart3
-import Risc0.Gadgets.OneHot20.Witness.WeakestPresPart4
-import Risc0.Gadgets.OneHot20.Witness.WeakestPresPart5
-import Risc0.Gadgets.OneHot20.Witness.WeakestPresPart6
-import Risc0.Gadgets.OneHot20.Witness.WeakestPresPart7
-import Risc0.Gadgets.OneHot20.Witness.WeakestPresPart8
-import Risc0.Gadgets.OneHot20.Witness.WeakestPresPart9
-import Risc0.Gadgets.OneHot20.Witness.WeakestPresPart10
-import Risc0.Gadgets.OneHot20.Witness.WeakestPresPart11
-import Risc0.Gadgets.OneHot20.Witness.WeakestPresPart12
-import Risc0.Gadgets.OneHot20.Witness.WeakestPresPart13
-import Risc0.Gadgets.OneHot20.Witness.WeakestPresPart14
-import Risc0.Gadgets.OneHot20.Witness.WeakestPresPart15
-import Risc0.Gadgets.OneHot20.Witness.WeakestPresPart16
-import Risc0.Gadgets.OneHot20.Witness.WeakestPresPart17
-import Risc0.Gadgets.OneHot20.Witness.WeakestPresPart18
-import Risc0.Gadgets.OneHot20.Witness.WeakestPresPart19
-import Risc0.Gadgets.OneHot20.Witness.WeakestPresPart20
-import Risc0.Gadgets.OneHot20.Witness.WeakestPresPart21
-import Risc0.Gadgets.OneHot20.Witness.WeakestPresPart22
-import Risc0.Gadgets.OneHot20.Witness.WeakestPresPart23
-import Risc0.Gadgets.OneHot20.Witness.WeakestPresPart24
-import Risc0.Gadgets.OneHot20.Witness.WeakestPresPart25
-import Risc0.Gadgets.OneHot20.Witness.WeakestPresPart26
-import Risc0.Gadgets.OneHot20.Witness.WeakestPresPart27
-import Risc0.Gadgets.OneHot20.Witness.WeakestPresPart28
-import Risc0.Gadgets.OneHot20.Witness.WeakestPresPart29
-import Risc0.Gadgets.OneHot20.Witness.WeakestPresPart30
-import Risc0.Gadgets.OneHot20.Witness.WeakestPresPart31
-import Risc0.Gadgets.OneHot20.Witness.WeakestPresPart32
-import Risc0.Gadgets.OneHot20.Witness.WeakestPresPart33
-import Risc0.Gadgets.OneHot20.Witness.WeakestPresPart34
-import Risc0.Gadgets.OneHot20.Witness.WeakestPresPart35
-import Risc0.Gadgets.OneHot20.Witness.WeakestPresPart36
-import Risc0.Gadgets.OneHot20.Witness.WeakestPresPart37
-import Risc0.Gadgets.OneHot20.Witness.WeakestPresPart38
-import Risc0.Gadgets.OneHot20.Witness.WeakestPresPart39
-import Risc0.Gadgets.OneHot20.Witness.WeakestPresPart40
-import Risc0.Gadgets.OneHot20.Witness.WeakestPresPart41
-import Risc0.Gadgets.OneHot20.Witness.WeakestPresPart42
-import Risc0.Gadgets.OneHot20.Witness.WeakestPresPart43
-import Risc0.Gadgets.OneHot20.Witness.WeakestPresPart44
-import Risc0.Gadgets.OneHot20.Witness.WeakestPresPart45
-import Risc0.Gadgets.OneHot20.Witness.WeakestPresPart46
-import Risc0.Gadgets.OneHot20.Witness.WeakestPresPart47
-import Risc0.Gadgets.OneHot20.Witness.WeakestPresPart48
-import Risc0.Gadgets.OneHot20.Witness.WeakestPresPart49
-import Risc0.Gadgets.OneHot20.Witness.WeakestPresPart50
-import Risc0.Gadgets.OneHot20.Witness.WeakestPresPart51
-import Risc0.Gadgets.OneHot20.Witness.WeakestPresPart52
-import Risc0.Gadgets.OneHot20.Witness.WeakestPresPart53
-import Risc0.Gadgets.OneHot20.Witness.WeakestPresPart54
+-- import Risc0.Gadgets.OneHot20.Witness.Code
+-- import Risc0.Gadgets.OneHot20.Constraints.Code
+-- import Risc0.Gadgets.OneHot20.Constraints.CodeReordered
+-- import Risc0.Gadgets.OneHot20.Witness.CodeReordered
+-- import Risc0.Gadgets.OneHot20.Constraints.CodeParts
+-- import Risc0.Gadgets.OneHot20.Witness.CodeParts
+-- import Risc0.Gadgets.OneHot20.Constraints.CodeDrops
+-- import Risc0.Gadgets.OneHot20.Witness.CodeDrops
+-- import Risc0.Gadgets.OneHot20.Constraints.WeakestPresPart0
+-- import Risc0.Gadgets.OneHot20.Constraints.WeakestPresPart1
+-- import Risc0.Gadgets.OneHot20.Constraints.WeakestPresPart2
+-- import Risc0.Gadgets.OneHot20.Constraints.WeakestPresPart3
+-- import Risc0.Gadgets.OneHot20.Constraints.WeakestPresPart4
+-- import Risc0.Gadgets.OneHot20.Constraints.WeakestPresPart5
+-- import Risc0.Gadgets.OneHot20.Constraints.WeakestPresPart6
+-- import Risc0.Gadgets.OneHot20.Constraints.WeakestPresPart7
+-- import Risc0.Gadgets.OneHot20.Constraints.WeakestPresPart8
+-- import Risc0.Gadgets.OneHot20.Constraints.WeakestPresPart9
+-- import Risc0.Gadgets.OneHot20.Constraints.WeakestPresPart10
+-- import Risc0.Gadgets.OneHot20.Constraints.WeakestPresPart11
+-- import Risc0.Gadgets.OneHot20.Constraints.WeakestPresPart12
+-- import Risc0.Gadgets.OneHot20.Constraints.WeakestPresPart13
+-- import Risc0.Gadgets.OneHot20.Constraints.WeakestPresPart14
+-- import Risc0.Gadgets.OneHot20.Constraints.WeakestPresPart15
+-- import Risc0.Gadgets.OneHot20.Constraints.WeakestPresPart16
+-- import Risc0.Gadgets.OneHot20.Constraints.WeakestPresPart17
+-- import Risc0.Gadgets.OneHot20.Constraints.WeakestPresPart18
+-- import Risc0.Gadgets.OneHot20.Constraints.WeakestPresPart19
+-- import Risc0.Gadgets.OneHot20.Constraints.WeakestPresPart20
+-- import Risc0.Gadgets.OneHot20.Constraints.WeakestPresPart21
+-- import Risc0.Gadgets.OneHot20.Constraints.WeakestPresPart22
+-- import Risc0.Gadgets.OneHot20.Constraints.WeakestPresPart23
+-- import Risc0.Gadgets.OneHot20.Constraints.WeakestPresPart24
+-- import Risc0.Gadgets.OneHot20.Constraints.WeakestPresPart25
+-- import Risc0.Gadgets.OneHot20.Constraints.WeakestPresPart26
+-- import Risc0.Gadgets.OneHot20.Constraints.WeakestPresPart27
+-- import Risc0.Gadgets.OneHot20.Constraints.WeakestPresPart28
+-- import Risc0.Gadgets.OneHot20.Constraints.WeakestPresPart29
+-- import Risc0.Gadgets.OneHot20.Constraints.WeakestPresPart30
+-- import Risc0.Gadgets.OneHot20.Constraints.WeakestPresPart31
+-- import Risc0.Gadgets.OneHot20.Constraints.WeakestPresPart32
+-- import Risc0.Gadgets.OneHot20.Constraints.WeakestPresPart33
+-- import Risc0.Gadgets.OneHot20.Constraints.WeakestPresPart34
+-- import Risc0.Gadgets.OneHot20.Constraints.WeakestPresPart35
+-- import Risc0.Gadgets.OneHot20.Constraints.WeakestPresPart36
+-- import Risc0.Gadgets.OneHot20.Constraints.WeakestPresPart37
+-- import Risc0.Gadgets.OneHot20.Constraints.WeakestPresPart38
+-- import Risc0.Gadgets.OneHot20.Constraints.WeakestPresPart39
+-- import Risc0.Gadgets.OneHot20.Witness.WeakestPresPart0
+-- import Risc0.Gadgets.OneHot20.Witness.WeakestPresPart1
+-- import Risc0.Gadgets.OneHot20.Witness.WeakestPresPart2
+-- import Risc0.Gadgets.OneHot20.Witness.WeakestPresPart3
+-- import Risc0.Gadgets.OneHot20.Witness.WeakestPresPart4
+-- import Risc0.Gadgets.OneHot20.Witness.WeakestPresPart5
+-- import Risc0.Gadgets.OneHot20.Witness.WeakestPresPart6
+-- import Risc0.Gadgets.OneHot20.Witness.WeakestPresPart7
+-- import Risc0.Gadgets.OneHot20.Witness.WeakestPresPart8
+-- import Risc0.Gadgets.OneHot20.Witness.WeakestPresPart9
+-- import Risc0.Gadgets.OneHot20.Witness.WeakestPresPart10
+-- import Risc0.Gadgets.OneHot20.Witness.WeakestPresPart11
+-- import Risc0.Gadgets.OneHot20.Witness.WeakestPresPart12
+-- import Risc0.Gadgets.OneHot20.Witness.WeakestPresPart13
+-- import Risc0.Gadgets.OneHot20.Witness.WeakestPresPart14
+-- import Risc0.Gadgets.OneHot20.Witness.WeakestPresPart15
+-- import Risc0.Gadgets.OneHot20.Witness.WeakestPresPart16
+-- import Risc0.Gadgets.OneHot20.Witness.WeakestPresPart17
+-- import Risc0.Gadgets.OneHot20.Witness.WeakestPresPart18
+-- import Risc0.Gadgets.OneHot20.Witness.WeakestPresPart19
+-- import Risc0.Gadgets.OneHot20.Witness.WeakestPresPart20
+-- import Risc0.Gadgets.OneHot20.Witness.WeakestPresPart21
+-- import Risc0.Gadgets.OneHot20.Witness.WeakestPresPart22
+-- import Risc0.Gadgets.OneHot20.Witness.WeakestPresPart23
+-- import Risc0.Gadgets.OneHot20.Witness.WeakestPresPart24
+-- import Risc0.Gadgets.OneHot20.Witness.WeakestPresPart25
+-- import Risc0.Gadgets.OneHot20.Witness.WeakestPresPart26
+-- import Risc0.Gadgets.OneHot20.Witness.WeakestPresPart27
+-- import Risc0.Gadgets.OneHot20.Witness.WeakestPresPart28
+-- import Risc0.Gadgets.OneHot20.Witness.WeakestPresPart29
+-- import Risc0.Gadgets.OneHot20.Witness.WeakestPresPart30
+-- import Risc0.Gadgets.OneHot20.Witness.WeakestPresPart31
+-- import Risc0.Gadgets.OneHot20.Witness.WeakestPresPart32
+-- import Risc0.Gadgets.OneHot20.Witness.WeakestPresPart33
+-- import Risc0.Gadgets.OneHot20.Witness.WeakestPresPart34
+-- import Risc0.Gadgets.OneHot20.Witness.WeakestPresPart35
+-- import Risc0.Gadgets.OneHot20.Witness.WeakestPresPart36
+-- import Risc0.Gadgets.OneHot20.Witness.WeakestPresPart37
+-- import Risc0.Gadgets.OneHot20.Witness.WeakestPresPart38
+-- import Risc0.Gadgets.OneHot20.Witness.WeakestPresPart39
+-- import Risc0.Gadgets.OneHot20.Witness.WeakestPresPart40
+-- import Risc0.Gadgets.OneHot20.Witness.WeakestPresPart41
+-- import Risc0.Gadgets.OneHot20.Witness.WeakestPresPart42
+-- import Risc0.Gadgets.OneHot20.Witness.WeakestPresPart43
+-- import Risc0.Gadgets.OneHot20.Witness.WeakestPresPart44
+-- import Risc0.Gadgets.OneHot20.Witness.WeakestPresPart45
+-- import Risc0.Gadgets.OneHot20.Witness.WeakestPresPart46
+-- import Risc0.Gadgets.OneHot20.Witness.WeakestPresPart47
+-- import Risc0.Gadgets.OneHot20.Witness.WeakestPresPart48
+-- import Risc0.Gadgets.OneHot20.Witness.WeakestPresPart49
+-- import Risc0.Gadgets.OneHot20.Witness.WeakestPresPart50
+-- import Risc0.Gadgets.OneHot20.Witness.WeakestPresPart51
+-- import Risc0.Gadgets.OneHot20.Witness.WeakestPresPart52
+-- import Risc0.Gadgets.OneHot20.Witness.WeakestPresPart53
+-- import Risc0.Gadgets.OneHot20.Witness.WeakestPresPart54
 
-import Risc0.Gadgets.IsZero.Witness.Code
-import Risc0.Gadgets.IsZero.Constraints.Code
-import Risc0.Gadgets.IsZero.Constraints.CodeReordered
-import Risc0.Gadgets.IsZero.Witness.CodeReordered
-import Risc0.Gadgets.IsZero.Constraints.CodeParts
-import Risc0.Gadgets.IsZero.Witness.CodeParts
-import Risc0.Gadgets.IsZero.Constraints.CodeDrops
-import Risc0.Gadgets.IsZero.Witness.CodeDrops
 import Risc0.Gadgets.IsZero.Constraints.WeakestPresPart0
 import Risc0.Gadgets.IsZero.Constraints.WeakestPresPart1
 import Risc0.Gadgets.IsZero.Constraints.WeakestPresPart2
 import Risc0.Gadgets.IsZero.Witness.WeakestPresPart0
 import Risc0.Gadgets.IsZero.Witness.WeakestPresPart1
 import Risc0.Gadgets.IsZero.Witness.WeakestPresPart2
-import Risc0.Gadgets.IsZero.Proofs
+-- import Risc0.Gadgets.IsZero.Proofs
 
-import Risc0.Gadgets.ComputeDecode.Witness.Code
-import Risc0.Gadgets.ComputeDecode.Constraints.Code
-import Risc0.Gadgets.ComputeDecode.Constraints.CodeReordered
-import Risc0.Gadgets.ComputeDecode.Witness.CodeReordered
-import Risc0.Gadgets.ComputeDecode.Constraints.CodeParts
-import Risc0.Gadgets.ComputeDecode.Witness.CodeParts
-import Risc0.Gadgets.ComputeDecode.Constraints.CodeDrops
-import Risc0.Gadgets.ComputeDecode.Witness.CodeDrops
-import Risc0.Gadgets.ComputeDecode.Constraints.WeakestPresPart0
-import Risc0.Gadgets.ComputeDecode.Constraints.WeakestPresPart1
-import Risc0.Gadgets.ComputeDecode.Constraints.WeakestPresPart2
-import Risc0.Gadgets.ComputeDecode.Constraints.WeakestPresPart3
-import Risc0.Gadgets.ComputeDecode.Constraints.WeakestPresPart4
-import Risc0.Gadgets.ComputeDecode.Constraints.WeakestPresPart5
-import Risc0.Gadgets.ComputeDecode.Constraints.WeakestPresPart6
-import Risc0.Gadgets.ComputeDecode.Constraints.WeakestPresPart7
-import Risc0.Gadgets.ComputeDecode.Constraints.WeakestPresPart8
-import Risc0.Gadgets.ComputeDecode.Constraints.WeakestPresPart9
-import Risc0.Gadgets.ComputeDecode.Constraints.WeakestPresPart10
-import Risc0.Gadgets.ComputeDecode.Constraints.WeakestPresPart11
-import Risc0.Gadgets.ComputeDecode.Constraints.WeakestPresPart12
-import Risc0.Gadgets.ComputeDecode.Constraints.WeakestPresPart13
-import Risc0.Gadgets.ComputeDecode.Constraints.WeakestPresPart14
-import Risc0.Gadgets.ComputeDecode.Constraints.WeakestPresPart15
-import Risc0.Gadgets.ComputeDecode.Constraints.WeakestPresPart16
-import Risc0.Gadgets.ComputeDecode.Witness.WeakestPresPart0
-import Risc0.Gadgets.ComputeDecode.Witness.WeakestPresPart1
-import Risc0.Gadgets.ComputeDecode.Witness.WeakestPresPart2
-import Risc0.Gadgets.ComputeDecode.Witness.WeakestPresPart3
-import Risc0.Gadgets.ComputeDecode.Witness.WeakestPresPart4
-import Risc0.Gadgets.ComputeDecode.Witness.WeakestPresPart5
-import Risc0.Gadgets.ComputeDecode.Witness.WeakestPresPart6
-import Risc0.Gadgets.ComputeDecode.Witness.WeakestPresPart7
-import Risc0.Gadgets.ComputeDecode.Witness.WeakestPresPart8
-import Risc0.Gadgets.ComputeDecode.Witness.WeakestPresPart9
-import Risc0.Gadgets.ComputeDecode.Witness.WeakestPresPart10
-import Risc0.Gadgets.ComputeDecode.Witness.WeakestPresPart11
-import Risc0.Gadgets.ComputeDecode.Witness.WeakestPresPart12
-import Risc0.Gadgets.ComputeDecode.Witness.WeakestPresPart13
-import Risc0.Gadgets.ComputeDecode.Witness.WeakestPresPart14
-import Risc0.Gadgets.ComputeDecode.Witness.WeakestPresPart15
-import Risc0.Gadgets.ComputeDecode.Witness.WeakestPresPart16
-import Risc0.Gadgets.ComputeDecode.Witness.WeakestPresPart17
-import Risc0.Gadgets.ComputeDecode.Witness.WeakestPresPart18
-import Risc0.Gadgets.ComputeDecode.Witness.WeakestPresPart19
-import Risc0.Gadgets.ComputeDecode.Witness.WeakestPresPart20
-import Risc0.Gadgets.ComputeDecode.Witness.WeakestPresPart21
-import Risc0.Gadgets.ComputeDecode.Witness.WeakestPresPart22
-import Risc0.Gadgets.ComputeDecode.Witness.WeakestPresPart23
-import Risc0.Gadgets.ComputeDecode.Witness.WeakestPresPart24
-import Risc0.Gadgets.ComputeDecode.Witness.WeakestPresPart25
-import Risc0.Gadgets.ComputeDecode.Witness.WeakestPresPart26
-import Risc0.Gadgets.ComputeDecode.Witness.WeakestPresPart27
-import Risc0.Gadgets.ComputeDecode.Witness.WeakestPresPart28
-import Risc0.Gadgets.ComputeDecode.Witness.WeakestPresPart29
-import Risc0.Gadgets.ComputeDecode.Witness.WeakestPresPart30
-import Risc0.Gadgets.ComputeDecode.Witness.WeakestPresPart31
+-- import Risc0.Gadgets.ComputeDecode.Constraints.WeakestPresPart0
+-- import Risc0.Gadgets.ComputeDecode.Constraints.WeakestPresPart1
+-- import Risc0.Gadgets.ComputeDecode.Constraints.WeakestPresPart2
+-- import Risc0.Gadgets.ComputeDecode.Constraints.WeakestPresPart3
+-- import Risc0.Gadgets.ComputeDecode.Constraints.WeakestPresPart4
+-- import Risc0.Gadgets.ComputeDecode.Constraints.WeakestPresPart5
+-- import Risc0.Gadgets.ComputeDecode.Constraints.WeakestPresPart6
+-- import Risc0.Gadgets.ComputeDecode.Constraints.WeakestPresPart7
+-- import Risc0.Gadgets.ComputeDecode.Constraints.WeakestPresPart8
+-- import Risc0.Gadgets.ComputeDecode.Constraints.WeakestPresPart9
+-- import Risc0.Gadgets.ComputeDecode.Constraints.WeakestPresPart10
+-- import Risc0.Gadgets.ComputeDecode.Constraints.WeakestPresPart11
+-- import Risc0.Gadgets.ComputeDecode.Constraints.WeakestPresPart12
+-- import Risc0.Gadgets.ComputeDecode.Constraints.WeakestPresPart13
+-- import Risc0.Gadgets.ComputeDecode.Constraints.WeakestPresPart14
+-- import Risc0.Gadgets.ComputeDecode.Constraints.WeakestPresPart15
+-- import Risc0.Gadgets.ComputeDecode.Constraints.WeakestPresPart16
+-- import Risc0.Gadgets.ComputeDecode.Witness.WeakestPresPart0
+-- import Risc0.Gadgets.ComputeDecode.Witness.WeakestPresPart1
+-- import Risc0.Gadgets.ComputeDecode.Witness.WeakestPresPart2
+-- import Risc0.Gadgets.ComputeDecode.Witness.WeakestPresPart3
+-- import Risc0.Gadgets.ComputeDecode.Witness.WeakestPresPart4
+-- import Risc0.Gadgets.ComputeDecode.Witness.WeakestPresPart5
+-- import Risc0.Gadgets.ComputeDecode.Witness.WeakestPresPart6
+-- import Risc0.Gadgets.ComputeDecode.Witness.WeakestPresPart7
+-- import Risc0.Gadgets.ComputeDecode.Witness.WeakestPresPart8
+-- import Risc0.Gadgets.ComputeDecode.Witness.WeakestPresPart9
+-- import Risc0.Gadgets.ComputeDecode.Witness.WeakestPresPart10
+-- import Risc0.Gadgets.ComputeDecode.Witness.WeakestPresPart11
+-- import Risc0.Gadgets.ComputeDecode.Witness.WeakestPresPart12
+-- import Risc0.Gadgets.ComputeDecode.Witness.WeakestPresPart13
+-- import Risc0.Gadgets.ComputeDecode.Witness.WeakestPresPart14
+-- import Risc0.Gadgets.ComputeDecode.Witness.WeakestPresPart15
+-- import Risc0.Gadgets.ComputeDecode.Witness.WeakestPresPart16
+-- import Risc0.Gadgets.ComputeDecode.Witness.WeakestPresPart17
+-- import Risc0.Gadgets.ComputeDecode.Witness.WeakestPresPart18
+-- import Risc0.Gadgets.ComputeDecode.Witness.WeakestPresPart19
+-- import Risc0.Gadgets.ComputeDecode.Witness.WeakestPresPart20
+-- import Risc0.Gadgets.ComputeDecode.Witness.WeakestPresPart21
+-- import Risc0.Gadgets.ComputeDecode.Witness.WeakestPresPart22
+-- import Risc0.Gadgets.ComputeDecode.Witness.WeakestPresPart23
+-- import Risc0.Gadgets.ComputeDecode.Witness.WeakestPresPart24
+-- import Risc0.Gadgets.ComputeDecode.Witness.WeakestPresPart25
+-- import Risc0.Gadgets.ComputeDecode.Witness.WeakestPresPart26
+-- import Risc0.Gadgets.ComputeDecode.Witness.WeakestPresPart27
+-- import Risc0.Gadgets.ComputeDecode.Witness.WeakestPresPart28
+-- import Risc0.Gadgets.ComputeDecode.Witness.WeakestPresPart29
+-- import Risc0.Gadgets.ComputeDecode.Witness.WeakestPresPart30
+-- import Risc0.Gadgets.ComputeDecode.Witness.WeakestPresPart31
 
 import Risc0.Gadgets.OneHot2.Witness.Code
 import Risc0.Gadgets.OneHot2.Constraints.Code
@@ -203,7 +187,7 @@ import Risc0.Gadgets.OneHot2.Witness.WeakestPresPart2
 import Risc0.Gadgets.OneHot2.Witness.WeakestPresPart3
 import Risc0.Gadgets.OneHot2.Witness.WeakestPresPart4
 import Risc0.Gadgets.OneHot2.Witness.WeakestPresPart5
-import Risc0.Gadgets.OneHot2.Proofs
+-- import Risc0.Gadgets.OneHot2.Proofs
 
 import Risc0.Gadgets.OneHot1.Witness.Code
 import Risc0.Gadgets.OneHot1.Constraints.Code
@@ -220,3 +204,19 @@ import Risc0.Gadgets.OneHot1.Witness.WeakestPresPart0
 import Risc0.Gadgets.OneHot1.Witness.WeakestPresPart1
 import Risc0.Gadgets.OneHot1.Witness.WeakestPresPart2
 import Risc0.Gadgets.OneHot1.Witness.WeakestPresPart3
+import Risc0.Gadgets.IsZero.Witness.Code
+import Risc0.Gadgets.IsZero.Constraints.Code
+import Risc0.Gadgets.IsZero.Constraints.CodeReordered
+import Risc0.Gadgets.IsZero.Witness.CodeReordered
+import Risc0.Gadgets.IsZero.Constraints.CodeParts
+import Risc0.Gadgets.IsZero.Witness.CodeParts
+import Risc0.Gadgets.IsZero.Constraints.CodeDrops
+import Risc0.Gadgets.IsZero.Witness.CodeDrops
+import Risc0.Gadgets.ComputeDecode.Witness.Code
+import Risc0.Gadgets.ComputeDecode.Constraints.Code
+import Risc0.Gadgets.ComputeDecode.Constraints.CodeReordered
+import Risc0.Gadgets.ComputeDecode.Witness.CodeReordered
+import Risc0.Gadgets.ComputeDecode.Constraints.CodeParts
+import Risc0.Gadgets.ComputeDecode.Witness.CodeParts
+import Risc0.Gadgets.ComputeDecode.Constraints.CodeDrops
+import Risc0.Gadgets.ComputeDecode.Witness.CodeDrops
