Risc0/Gadgets/IsZero/Witness/WeakestPresPart0.lean
@@ -59,6 +59,7 @@ lemma part0_wp {st : State} {data0 data1 : Option Felt} :
   unfold part0_state_update part0_drops part0_state
   rfl
 
+set_option maxRecDepth 10000000 in
 lemma part0_cumulative_wp {in0: Felt} {data0 data1: Option Felt} :
   Code.run (start_state ([in0])) ([data0, data1]) ↔
   Code.getReturn
