Risc0/Gadgets/OneHot1/Witness/CodeDrops.lean
@@ -17,7 +17,7 @@ lemma drop_past_part1 (h0: ⟨"%1"⟩ ≠ x) (h1: ⟨"%2"⟩ ≠ x) (h2: ⟨"%3"
     rewrite [←drop_sequencing_dddd]
     rewrite [h_rhs]
     unfold part1
-    rfl
+    simp only [MLIR.run_seq_def]; try rfl
 lemma drop_past_part2 (h0: ⟨"%0"⟩ ≠ x) (h1: ⟨"%4"⟩ ≠ x) (h2: ⟨"%5"⟩ ≠ x) (h3: ⟨"%6"⟩ ≠ x) (h4: ⟨"%7"⟩ ≠ x):
   (Γ st ⟦dropfelt x; part2; rest⟧) =
   (Γ st ⟦part2; dropfelt x; rest⟧) := by
@@ -31,7 +31,7 @@ lemma drop_past_part2 (h0: ⟨"%0"⟩ ≠ x) (h1: ⟨"%4"⟩ ≠ x) (h2: ⟨"%5"
     rewrite [←drop_sequencing_dddd]
     rewrite [h_rhs]
     unfold part2
-    rfl
+    simp only [MLIR.run_seq_def]; try rfl
 lemma drop_past_part3 (h0: ⟨"%7"⟩ ≠ x):
   (Γ st ⟦dropfelt x; part3; rest⟧) =
   (Γ st ⟦part3; dropfelt x; rest⟧) := by
@@ -45,7 +45,7 @@ lemma drop_past_part3 (h0: ⟨"%7"⟩ ≠ x):
     rewrite [←drop_sequencing_d]
     rewrite [h_rhs]
     unfold part3
-    rfl
+    simp only [MLIR.run_seq_def]; try rfl
 
 lemma behaviour_with_drops3 :
   Γ st ⟦dropfelt ⟨"%8"⟩;dropfelt ⟨"%2"⟩;dropfelt ⟨"%1"⟩;dropfelt ⟨"%3"⟩;dropfelt ⟨"%0"⟩;dropfelt ⟨"%4"⟩;dropfelt ⟨"%5"⟩;dropfelt ⟨"%6"⟩;part3;dropfelt ⟨"%7"⟩⟧ =
@@ -54,7 +54,7 @@ lemma behaviour_with_drops3 :
     rewrite [drop_past_part3 (by trivial), ←MLIR.run_seq_def,drop_past_part3 (by trivial), ←MLIR.run_seq_def,drop_past_part3 (by trivial), ←MLIR.run_seq_def,drop_past_part3 (by trivial), ←MLIR.run_seq_def,drop_past_part3 (by trivial), ←MLIR.run_seq_def,drop_past_part3 (by trivial), ←MLIR.run_seq_def,drop_past_part3 (by trivial), ←MLIR.run_seq_def]
     rewrite [drop_past_part3 (by trivial), MLIR.run_seq_def]
     rewrite [←MLIR.run_seq_def]
-    rfl
+    simp only [MLIR.run_seq_def]; try rfl
 lemma behaviour_with_drops2 :
   Γ st ⟦dropfelt ⟨"%8"⟩;dropfelt ⟨"%2"⟩;dropfelt ⟨"%1"⟩;dropfelt ⟨"%3"⟩;part2;dropfelt ⟨"%0"⟩;dropfelt ⟨"%4"⟩;dropfelt ⟨"%5"⟩;dropfelt ⟨"%6"⟩;part3;dropfelt ⟨"%7"⟩⟧ =
   Γ st ⟦part2;part3;dropfelt ⟨"%8"⟩;dropfelt ⟨"%2"⟩;dropfelt ⟨"%1"⟩;dropfelt ⟨"%3"⟩;dropfelt ⟨"%0"⟩;dropfelt ⟨"%4"⟩;dropfelt ⟨"%5"⟩;dropfelt ⟨"%6"⟩;dropfelt ⟨"%7"⟩⟧ := by
@@ -62,19 +62,19 @@ lemma behaviour_with_drops2 :
     rewrite [drop_past_part2 (by trivial) (by trivial) (by trivial) (by trivial) (by trivial), ←MLIR.run_seq_def,drop_past_part2 (by trivial) (by trivial) (by trivial) (by trivial) (by trivial), ←MLIR.run_seq_def,drop_past_part2 (by trivial) (by trivial) (by trivial) (by trivial) (by trivial), ←MLIR.run_seq_def]
     rewrite [drop_past_part2 (by trivial) (by trivial) (by trivial) (by trivial) (by trivial), MLIR.run_seq_def]
     rewrite [behaviour_with_drops3, ←MLIR.run_seq_def]
-    rfl
+    simp only [MLIR.run_seq_def]; try rfl
 lemma behaviour_with_drops1 :
   Γ st ⟦dropfelt ⟨"%8"⟩;part1;dropfelt ⟨"%2"⟩;dropfelt ⟨"%1"⟩;dropfelt ⟨"%3"⟩;part2;dropfelt ⟨"%0"⟩;dropfelt ⟨"%4"⟩;dropfelt ⟨"%5"⟩;dropfelt ⟨"%6"⟩;part3;dropfelt ⟨"%7"⟩⟧ =
   Γ st ⟦part1;part2;part3;dropfelt ⟨"%8"⟩;dropfelt ⟨"%2"⟩;dropfelt ⟨"%1"⟩;dropfelt ⟨"%3"⟩;dropfelt ⟨"%0"⟩;dropfelt ⟨"%4"⟩;dropfelt ⟨"%5"⟩;dropfelt ⟨"%6"⟩;dropfelt ⟨"%7"⟩⟧ := by
     rewrite [drop_past_part1 (by trivial) (by trivial) (by trivial) (by trivial) (by trivial), MLIR.run_seq_def]
     rewrite [behaviour_with_drops2, ←MLIR.run_seq_def]
-    rfl
+    simp only [MLIR.run_seq_def]; try rfl
 lemma behaviour_with_drops :
   Γ st ⟦part0;dropfelt ⟨"%8"⟩;part1;dropfelt ⟨"%2"⟩;dropfelt ⟨"%1"⟩;dropfelt ⟨"%3"⟩;part2;dropfelt ⟨"%0"⟩;dropfelt ⟨"%4"⟩;dropfelt ⟨"%5"⟩;dropfelt ⟨"%6"⟩;part3;dropfelt ⟨"%7"⟩⟧ =
   Γ st ⟦part0;part1;part2;part3;dropfelt ⟨"%8"⟩;dropfelt ⟨"%2"⟩;dropfelt ⟨"%1"⟩;dropfelt ⟨"%3"⟩;dropfelt ⟨"%0"⟩;dropfelt ⟨"%4"⟩;dropfelt ⟨"%5"⟩;dropfelt ⟨"%6"⟩;dropfelt ⟨"%7"⟩⟧ := by
     rewrite [MLIR.run_seq_def]
     rewrite [behaviour_with_drops1, ←MLIR.run_seq_def]
-    rfl
+    simp only [MLIR.run_seq_def]; try rfl
 lemma getReturn_ignores_drops :
   getReturn (Γ st ⟦part0;part1;part2;part3;dropfelt ⟨"%8"⟩;dropfelt ⟨"%2"⟩;dropfelt ⟨"%1"⟩;dropfelt ⟨"%3"⟩;dropfelt ⟨"%0"⟩;dropfelt ⟨"%4"⟩;dropfelt ⟨"%5"⟩;dropfelt ⟨"%6"⟩;dropfelt ⟨"%7"⟩⟧) res0 =
   getReturn (Γ st ⟦part0;part1;part2;part3⟧) res0 := by
