Risc0/Gadgets/OneHot1/Witness/WeakestPresPart0.lean
@@ -49,6 +49,7 @@ lemma part0_wp {st : State} {data0 : Option Felt} :
   unfold part0_state_update part0_drops part0_state
   rfl
 
+set_option maxRecDepth 10000000 in
 lemma part0_cumulative_wp {code0: Felt} {data0: Option Felt} :
   Code.run (start_state ([code0])) ([data0]) ↔
   Code.getReturn
