Risc0/Gadgets/OneHot2/Witness/CodeDrops.lean
@@ -17,7 +17,7 @@ lemma drop_past_part1 (h0: ⟨"%2"⟩ ≠ x) (h1: ⟨"%0"⟩ ≠ x) (h2: ⟨"%13
     rewrite [←drop_sequencing_nnnd]
     rewrite [h_rhs]
     unfold part1
-    rfl
+    simp only [MLIR.run_seq_def]; try rfl
 lemma drop_past_part2 (h0: ⟨"%3"⟩ ≠ x) (h1: ⟨"%2"⟩ ≠ x) (h2: ⟨"%4"⟩ ≠ x) (h3: ⟨"%5"⟩ ≠ x) (h4: ⟨"%0"⟩ ≠ x) (h5: ⟨"%6"⟩ ≠ x):
   (Γ st ⟦dropfelt x; part2; rest⟧) =
   (Γ st ⟦part2; dropfelt x; rest⟧) := by
@@ -31,7 +31,7 @@ lemma drop_past_part2 (h0: ⟨"%3"⟩ ≠ x) (h1: ⟨"%2"⟩ ≠ x) (h2: ⟨"%4"
     rewrite [←drop_sequencing_dddd]
     rewrite [h_rhs]
     unfold part2
-    rfl
+    simp only [MLIR.run_seq_def]; try rfl
 lemma drop_past_part3 (h0: ⟨"%5"⟩ ≠ x) (h1: ⟨"%6"⟩ ≠ x) (h2: ⟨"%7"⟩ ≠ x) (h3: ⟨"%0"⟩ ≠ x) (h4: ⟨"%3"⟩ ≠ x) (h5: ⟨"%8"⟩ ≠ x) (h6: ⟨"%9"⟩ ≠ x):
   (Γ st ⟦dropfelt x; part3; rest⟧) =
   (Γ st ⟦part3; dropfelt x; rest⟧) := by
@@ -45,7 +45,7 @@ lemma drop_past_part3 (h0: ⟨"%5"⟩ ≠ x) (h1: ⟨"%6"⟩ ≠ x) (h2: ⟨"%7"
     rewrite [←drop_sequencing_dddd]
     rewrite [h_rhs]
     unfold part3
-    rfl
+    simp only [MLIR.run_seq_def]; try rfl
 lemma drop_past_part4 (h0: ⟨"%9"⟩ ≠ x) (h1: ⟨"%5"⟩ ≠ x) (h2: ⟨"%3"⟩ ≠ x) (h3: ⟨"%10"⟩ ≠ x) (h4: ⟨"%0"⟩ ≠ x) (h5: ⟨"%11"⟩ ≠ x) (h6: ⟨"%1"⟩ ≠ x):
   (Γ st ⟦dropfelt x; part4; rest⟧) =
   (Γ st ⟦part4; dropfelt x; rest⟧) := by
@@ -59,7 +59,7 @@ lemma drop_past_part4 (h0: ⟨"%9"⟩ ≠ x) (h1: ⟨"%5"⟩ ≠ x) (h2: ⟨"%3"
     rewrite [←drop_sequencing_dddd]
     rewrite [h_rhs]
     unfold part4
-    rfl
+    simp only [MLIR.run_seq_def]; try rfl
 lemma drop_past_part5 (h0: ⟨"%11"⟩ ≠ x):
   (Γ st ⟦dropfelt x; part5; rest⟧) =
   (Γ st ⟦part5; dropfelt x; rest⟧) := by
@@ -73,7 +73,7 @@ lemma drop_past_part5 (h0: ⟨"%11"⟩ ≠ x):
     rewrite [←drop_sequencing_d]
     rewrite [h_rhs]
     unfold part5
-    rfl
+    simp only [MLIR.run_seq_def]; try rfl
 
 lemma behaviour_with_drops5_1 :
   Γ st ⟦dropfelt ⟨"%2"⟩;dropfelt ⟨"%4"⟩;dropfelt ⟨"%6"⟩;dropfelt ⟨"%7"⟩;dropfelt ⟨"%8"⟩;dropfelt ⟨"%0"⟩;dropfelt ⟨"%3"⟩;dropfelt ⟨"%5"⟩;dropfelt ⟨"%9"⟩;dropfelt ⟨"%10"⟩;part5;rest⟧ =
@@ -89,7 +89,7 @@ lemma behaviour_with_drops5 :
     rewrite [drop_past_part5 (by trivial), ←MLIR.run_seq_def,drop_past_part5 (by trivial), ←MLIR.run_seq_def]
     rewrite [drop_past_part5 (by trivial), MLIR.run_seq_def]
     rewrite [←MLIR.run_seq_def]
-    rfl
+    simp only [MLIR.run_seq_def]; try rfl
 lemma behaviour_with_drops4 :
   Γ st ⟦dropfelt ⟨"%12"⟩;dropfelt ⟨"%13"⟩;dropfelt ⟨"%14"⟩;dropfelt ⟨"%2"⟩;dropfelt ⟨"%4"⟩;dropfelt ⟨"%6"⟩;dropfelt ⟨"%7"⟩;dropfelt ⟨"%8"⟩;part4;dropfelt ⟨"%0"⟩;dropfelt ⟨"%3"⟩;dropfelt ⟨"%5"⟩;dropfelt ⟨"%9"⟩;dropfelt ⟨"%10"⟩;part5;dropfelt ⟨"%11"⟩;dropfelt ⟨"%1"⟩⟧ =
   Γ st ⟦part4;part5;dropfelt ⟨"%12"⟩;dropfelt ⟨"%13"⟩;dropfelt ⟨"%14"⟩;dropfelt ⟨"%2"⟩;dropfelt ⟨"%4"⟩;dropfelt ⟨"%6"⟩;dropfelt ⟨"%7"⟩;dropfelt ⟨"%8"⟩;dropfelt ⟨"%0"⟩;dropfelt ⟨"%3"⟩;dropfelt ⟨"%5"⟩;dropfelt ⟨"%9"⟩;dropfelt ⟨"%10"⟩;dropfelt ⟨"%11"⟩;dropfelt ⟨"%1"⟩⟧ := by
@@ -97,7 +97,7 @@ lemma behaviour_with_drops4 :
     rewrite [drop_past_part4 (by trivial) (by trivial) (by trivial) (by trivial) (by trivial) (by trivial) (by trivial), ←MLIR.run_seq_def,drop_past_part4 (by trivial) (by trivial) (by trivial) (by trivial) (by trivial) (by trivial) (by trivial), ←MLIR.run_seq_def,drop_past_part4 (by trivial) (by trivial) (by trivial) (by trivial) (by trivial) (by trivial) (by trivial), ←MLIR.run_seq_def,drop_past_part4 (by trivial) (by trivial) (by trivial) (by trivial) (by trivial) (by trivial) (by trivial), ←MLIR.run_seq_def,drop_past_part4 (by trivial) (by trivial) (by trivial) (by trivial) (by trivial) (by trivial) (by trivial), ←MLIR.run_seq_def,drop_past_part4 (by trivial) (by trivial) (by trivial) (by trivial) (by trivial) (by trivial) (by trivial), ←MLIR.run_seq_def,drop_past_part4 (by trivial) (by trivial) (by trivial) (by trivial) (by trivial) (by trivial) (by trivial), ←MLIR.run_seq_def]
     rewrite [drop_past_part4 (by trivial) (by trivial) (by trivial) (by trivial) (by trivial) (by trivial) (by trivial), MLIR.run_seq_def]
     rewrite [behaviour_with_drops5, ←MLIR.run_seq_def]
-    rfl
+    simp only [MLIR.run_seq_def]; try rfl
 lemma behaviour_with_drops3 :
   Γ st ⟦dropfelt ⟨"%12"⟩;dropfelt ⟨"%13"⟩;dropfelt ⟨"%14"⟩;dropfelt ⟨"%2"⟩;dropfelt ⟨"%4"⟩;part3;dropfelt ⟨"%6"⟩;dropfelt ⟨"%7"⟩;dropfelt ⟨"%8"⟩;part4;dropfelt ⟨"%0"⟩;dropfelt ⟨"%3"⟩;dropfelt ⟨"%5"⟩;dropfelt ⟨"%9"⟩;dropfelt ⟨"%10"⟩;part5;dropfelt ⟨"%11"⟩;dropfelt ⟨"%1"⟩⟧ =
   Γ st ⟦part3;part4;part5;dropfelt ⟨"%12"⟩;dropfelt ⟨"%13"⟩;dropfelt ⟨"%14"⟩;dropfelt ⟨"%2"⟩;dropfelt ⟨"%4"⟩;dropfelt ⟨"%6"⟩;dropfelt ⟨"%7"⟩;dropfelt ⟨"%8"⟩;dropfelt ⟨"%0"⟩;dropfelt ⟨"%3"⟩;dropfelt ⟨"%5"⟩;dropfelt ⟨"%9"⟩;dropfelt ⟨"%10"⟩;dropfelt ⟨"%11"⟩;dropfelt ⟨"%1"⟩⟧ := by
@@ -105,7 +105,7 @@ lemma behaviour_with_drops3 :
     rewrite [drop_past_part3 (by trivial) (by trivial) (by trivial) (by trivial) (by trivial) (by trivial) (by trivial), ←MLIR.run_seq_def,drop_past_part3 (by trivial) (by trivial) (by trivial) (by trivial) (by trivial) (by trivial) (by trivial), ←MLIR.run_seq_def,drop_past_part3 (by trivial) (by trivial) (by trivial) (by trivial) (by trivial) (by trivial) (by trivial), ←MLIR.run_seq_def,drop_past_part3 (by trivial) (by trivial) (by trivial) (by trivial) (by trivial) (by trivial) (by trivial), ←MLIR.run_seq_def]
     rewrite [drop_past_part3 (by trivial) (by trivial) (by trivial) (by trivial) (by trivial) (by trivial) (by trivial), MLIR.run_seq_def]
     rewrite [behaviour_with_drops4, ←MLIR.run_seq_def]
-    rfl
+    simp only [MLIR.run_seq_def]; try rfl
 lemma behaviour_with_drops2 :
   Γ st ⟦dropfelt ⟨"%12"⟩;dropfelt ⟨"%13"⟩;dropfelt ⟨"%14"⟩;part2;dropfelt ⟨"%2"⟩;dropfelt ⟨"%4"⟩;part3;dropfelt ⟨"%6"⟩;dropfelt ⟨"%7"⟩;dropfelt ⟨"%8"⟩;part4;dropfelt ⟨"%0"⟩;dropfelt ⟨"%3"⟩;dropfelt ⟨"%5"⟩;dropfelt ⟨"%9"⟩;dropfelt ⟨"%10"⟩;part5;dropfelt ⟨"%11"⟩;dropfelt ⟨"%1"⟩⟧ =
   Γ st ⟦part2;part3;part4;part5;dropfelt ⟨"%12"⟩;dropfelt ⟨"%13"⟩;dropfelt ⟨"%14"⟩;dropfelt ⟨"%2"⟩;dropfelt ⟨"%4"⟩;dropfelt ⟨"%6"⟩;dropfelt ⟨"%7"⟩;dropfelt ⟨"%8"⟩;dropfelt ⟨"%0"⟩;dropfelt ⟨"%3"⟩;dropfelt ⟨"%5"⟩;dropfelt ⟨"%9"⟩;dropfelt ⟨"%10"⟩;dropfelt ⟨"%11"⟩;dropfelt ⟨"%1"⟩⟧ := by
@@ -113,19 +113,19 @@ lemma behaviour_with_drops2 :
     rewrite [drop_past_part2 (by trivial) (by trivial) (by trivial) (by trivial) (by trivial) (by trivial), ←MLIR.run_seq_def,drop_past_part2 (by trivial) (by trivial) (by trivial) (by trivial) (by trivial) (by trivial), ←MLIR.run_seq_def]
     rewrite [drop_past_part2 (by trivial) (by trivial) (by trivial) (by trivial) (by trivial) (by trivial), MLIR.run_seq_def]
     rewrite [behaviour_with_drops3, ←MLIR.run_seq_def]
-    rfl
+    simp only [MLIR.run_seq_def]; try rfl
 lemma behaviour_with_drops1 :
   Γ st ⟦dropfelt ⟨"%12"⟩;part1;dropfelt ⟨"%13"⟩;dropfelt ⟨"%14"⟩;part2;dropfelt ⟨"%2"⟩;dropfelt ⟨"%4"⟩;part3;dropfelt ⟨"%6"⟩;dropfelt ⟨"%7"⟩;dropfelt ⟨"%8"⟩;part4;dropfelt ⟨"%0"⟩;dropfelt ⟨"%3"⟩;dropfelt ⟨"%5"⟩;dropfelt ⟨"%9"⟩;dropfelt ⟨"%10"⟩;part5;dropfelt ⟨"%11"⟩;dropfelt ⟨"%1"⟩⟧ =
   Γ st ⟦part1;part2;part3;part4;part5;dropfelt ⟨"%12"⟩;dropfelt ⟨"%13"⟩;dropfelt ⟨"%14"⟩;dropfelt ⟨"%2"⟩;dropfelt ⟨"%4"⟩;dropfelt ⟨"%6"⟩;dropfelt ⟨"%7"⟩;dropfelt ⟨"%8"⟩;dropfelt ⟨"%0"⟩;dropfelt ⟨"%3"⟩;dropfelt ⟨"%5"⟩;dropfelt ⟨"%9"⟩;dropfelt ⟨"%10"⟩;dropfelt ⟨"%11"⟩;dropfelt ⟨"%1"⟩⟧ := by
     rewrite [drop_past_part1 (by trivial) (by trivial) (by trivial) (by trivial) (by trivial), MLIR.run_seq_def]
     rewrite [behaviour_with_drops2, ←MLIR.run_seq_def]
-    rfl
+    simp only [MLIR.run_seq_def]; try rfl
 lemma behaviour_with_drops :
   Γ st ⟦part0;dropfelt ⟨"%12"⟩;part1;dropfelt ⟨"%13"⟩;dropfelt ⟨"%14"⟩;part2;dropfelt ⟨"%2"⟩;dropfelt ⟨"%4"⟩;part3;dropfelt ⟨"%6"⟩;dropfelt ⟨"%7"⟩;dropfelt ⟨"%8"⟩;part4;dropfelt ⟨"%0"⟩;dropfelt ⟨"%3"⟩;dropfelt ⟨"%5"⟩;dropfelt ⟨"%9"⟩;dropfelt ⟨"%10"⟩;part5;dropfelt ⟨"%11"⟩;dropfelt ⟨"%1"⟩⟧ =
   Γ st ⟦part0;part1;part2;part3;part4;part5;dropfelt ⟨"%12"⟩;dropfelt ⟨"%13"⟩;dropfelt ⟨"%14"⟩;dropfelt ⟨"%2"⟩;dropfelt ⟨"%4"⟩;dropfelt ⟨"%6"⟩;dropfelt ⟨"%7"⟩;dropfelt ⟨"%8"⟩;dropfelt ⟨"%0"⟩;dropfelt ⟨"%3"⟩;dropfelt ⟨"%5"⟩;dropfelt ⟨"%9"⟩;dropfelt ⟨"%10"⟩;dropfelt ⟨"%11"⟩;dropfelt ⟨"%1"⟩⟧ := by
     rewrite [MLIR.run_seq_def]
     rewrite [behaviour_with_drops1, ←MLIR.run_seq_def]
-    rfl
+    simp only [MLIR.run_seq_def]; try rfl
 lemma getReturn_ignores_drops :
   getReturn (Γ st ⟦part0;part1;part2;part3;part4;part5;dropfelt ⟨"%12"⟩;dropfelt ⟨"%13"⟩;dropfelt ⟨"%14"⟩;dropfelt ⟨"%2"⟩;dropfelt ⟨"%4"⟩;dropfelt ⟨"%6"⟩;dropfelt ⟨"%7"⟩;dropfelt ⟨"%8"⟩;dropfelt ⟨"%0"⟩;dropfelt ⟨"%3"⟩;dropfelt ⟨"%5"⟩;dropfelt ⟨"%9"⟩;dropfelt ⟨"%10"⟩;dropfelt ⟨"%11"⟩;dropfelt ⟨"%1"⟩⟧) res0 =
   getReturn (Γ st ⟦part0;part1;part2;part3;part4;part5⟧) res0 := by
