Risc0/Gadgets/OneHot2/Witness/WeakestPresPart4.lean
@@ -44,6 +44,7 @@ lemma part4_updates_opaque {st : State} :
   Code.getReturn (part4_state_update (part3_drops (part3_state st))) ([data0, data1]) := by
   simp [part3_state_update, part4_wp]
 
+set_option maxRecDepth 10000000 in
 lemma part4_cumulative_wp {code0: Felt} {data0 data1: Option Felt} :
   Code.run (start_state ([code0])) ([data0, data1]) ↔
   Code.getReturn
