Risc0/State/Init.lean
@@ -44,12 +44,12 @@ namespace Risc0.State
     init numInput numOutput
           ((Buffer.init numInput).head (by simp [Buffer.init]))
           ((Buffer.init numOutput).head (by simp [Buffer.init]))
-          (by simp [Buffer.init])
-          (by simp [Buffer.init])
+          (by simp [Buffer.init, BufferAtTime.init])
+          (by simp [Buffer.init, BufferAtTime.init])
 
   private lemma valid_init'_aux :
     bufferLensConsistent (State.init m n input output hIn hOut) := λ var h h₁ row h₂ => by
-    simp [bufferWidths, init, Buffer.init']
+    simp [bufferWidths, init, Buffer.init', BufferAtTime.init]
     have : var = ⟨Input⟩ ∨ var = ⟨Output⟩ := by
       unfold init at h; rw [Map.mem_fromList] at h; simp at h; exact h
     have : row = 0 := by simp [init] at h₂; exact h₂
